src/algebras/dill.v
@@ -1,16 +1,16 @@
 From Hammer Require Import Hammer.
 From VST.msl Require Import sepalg sepalg_generators.
-From CARVe.algebras Require Import purely_linear structural.
+From CARVe.algebras Require Import linear structural.
 
-Definition mult : Type := purely_linear.mult + structural.mult.
+Definition mult : Type := linear.mult + structural.mult.
 
 (* Handy definitions *)
-Definition zero  : mult := inl purely_linear.zero.
-Definition one   : mult := inl purely_linear.one.
+Definition zero  : mult := inl linear.zero.
+Definition one   : mult := inl linear.one.
 Definition omega : mult := inr tt.
 
 Instance Join_mult : Join mult :=
-  Join_sum _ purely_linear.Join_mult _ structural.Join_mult.
+  Join_sum _ linear.Join_mult _ structural.Join_mult.
 
 (* The following definition and lemma are an inductive
 characterization of the join that MSL generates. They exists solely to
@@ -25,15 +25,13 @@ Inductive mult_op : mult -> mult -> mult -> Prop:=
 
 Lemma join_is_mult_op : forall (x y z : mult),
     join x y z <-> mult_op x y z.
-Proof.
-  sauto.
-Qed.
+Proof. sauto. Qed.
 
 Instance mult_Perm_alg : Perm_alg mult :=
-  Perm_sum _ _ _ _ purely_linear.Perm_alg_mult structural.Perm_mult.
+  Perm_sum _ _ _ _ linear.Perm_alg_mult structural.Perm_mult.
 
 Instance mult_Sep_alg : Sep_alg mult :=
-  Sep_sum _ _ _ _ _ _ purely_linear.mult_Sep_alg structural.Sep_mult.
+  Sep_sum _ _ _ _ _ _ linear.mult_Sep_alg structural.Sep_mult.
 
 Variant hal : mult -> Prop :=
   | halz : hal zero
@@ -42,6 +40,4 @@ Variant hal : mult -> Prop :=
 Definition hal_core : mult -> Prop := fun m => m = (core m).
 
 Lemma hal_is_core : forall x, hal x <-> hal_core x.
-Proof.
-  sauto.
-Qed.
+Proof. sauto. Qed.
