src/contexts/list.v
@@ -14,180 +14,414 @@
   free properties like commutativity, associativity, cancellativity, etc.
 **)
 
-From Coq Require Import List Program.Equality.
-From Hammer Require Import Tactics.
-From VST.msl Require Import sepalg sepalg_generators.
+From Coq Require Import List Program.Equality Sorting.Permutation Unicode.Utf8.
+From Hammer Require Import Hammer.
 Import List.ListNotations.
+From VST.msl Require Import sepalg sepalg_generators.
 
 Section ListCtx.
 
-  Variable R : Type. (* Resources *)
-  Variable A : Type. (* Resource Algebra *)
-  Variable JA : Join A.
-  Variable CA : Canc_alg A.
-  Variable PA : Perm_alg A.
-  Variable SA : Sep_alg A.
+  Variable R: Type. (* Resources *)
+  Variable A: Type. (* Resource algebra *)
+  Variable JA: Join A.
+  Variable CA: Canc_alg A.
+  Variable PA: Perm_alg A.
+  Variable SA: Sep_alg A.
 
   (* Functor from permission algebras A to contexts of resources of
     type R, i.e., to list (R * A). *)
   Definition lctx : Type := list (R * A).
 
+  (* Hypothesis eq_dec : forall x y : A, {x = y} + {x <> y}. *)
+
+  (* ---------------- Algebraic structure ---------------- *)
+
   #[global] Instance Join_lctx : Join lctx :=
     Join_list _ (Join_prod _ (Join_equiv _) _ JA).
 
   #[global] Instance Perm_alg_lctx : Perm_alg lctx.
-  Proof.
-    sauto use: Perm_list, Perm_prod, Perm_equiv.
-  Qed.
+  Proof. sauto use: Perm_list, Perm_prod, Perm_equiv. Qed.
 
   #[global] Instance Canc_alg_lctx : Canc_alg lctx.
-  Proof.
-    intros; apply Canc_list, Canc_prod; [ apply Canc_equiv | auto ].
-  Qed.
+  Proof. intros; apply Canc_list, Canc_prod; [ apply Canc_equiv | auto ]. Qed.
 
   #[global] Instance Sep_alg_lctx : Sep_alg lctx.
+  Proof. intros; apply Sep_list, Sep_prod; sauto. Qed.
+
+  (* ---------------- Exhaustedness ---------------- *)
+
+  (* Exhaustedness as a functional program *)
+  Definition exh (hal : A -> Prop) : lctx -> Prop :=
+    fold_right (fun ra p => and (hal (snd ra)) p) True.
+
+  (* Exhaustedness as an inductive predicate *)
+  Inductive exh_ind (hal : A -> Prop) : lctx -> Prop :=
+  | exh_ind_n : exh_ind hal []
+  | exh_ind_c {l a} :
+    forall r, exh_ind hal l -> hal a -> exh_ind hal ((r, a) :: l).
+
+  (* Equivalence of functional and inductive definitions *)
+  Lemma exh_ind_iff hal l :
+    exh_ind hal l <-> exh hal l.
   Proof.
-    intros; apply Sep_list, Sep_prod; sauto.
+    split.
+    - induction 1; simpl; auto.
+    - induction l as [|[? ?] ? ?]; intros H; constructor; destruct H; auto.
   Qed.
 
-End ListCtx.
+  (* ---------------- Lookup / update ---------------- *)
 
-(* -------------------------------------------- *)
-(* Inductive characterization of merge          *)
-(* -------------------------------------------- *)
+  Definition lookup (l : lctx) (n : nat) : option (R * A) := nth_error l n.
 
-(**
-  As a sanity check, we give an inductive characterization of lctx,
-  and show that it has the same action on the join relation. We should
-  not directly use this definition in any future developments, but
-  instead should use JoinFunctor_lctx applied to the resource algebra we are
-  annotating contexts with.
-**)
+  Definition has_entry (l : lctx) (x : R * A) : Prop := In x l.
 
-Inductive merge {R A: Type} {join: Join A} : Join (lctx R A) :=
-| mg_n : merge [] [] []
-| mg_c r {Δ₁ Δ₂ Δ α₁ α₂ α} :
-    join α₁ α₂ α ->
-    merge Δ₁ Δ₂ Δ ->
-    merge ((r, α₁) :: Δ₁) ((r, α₂) :: Δ₂) ((r, α) :: Δ).
+  Fixpoint upd (l : lctx) (n : nat) (x : R * A) : lctx :=
+    match n, l with
+    | _, [] => []
+    | 0, _ :: tl => x :: tl
+    | S n', hd :: tl => hd :: upd tl n' x
+    end.
+  
+  (* Update as a relation *)
+  Inductive upd_rel : lctx -> nat -> R * A -> R * A -> lctx -> Prop :=
+  | updrel_t : forall (l : lctx) x y,
+    upd_rel (x :: l) 0 x y (y :: l)
+  | updrel_n {l l' n x x' y} :
+    upd_rel l n x x' l' ->
+    upd_rel (y :: l) (S n) x x' (y :: l').
 
-Proposition merge_is_JoinFunctor_lctx
-  {A R: Type} {JA: Join A} {L1 L2 L3 : list (R * A)}:
-    merge L1 L2 L3 <-> join L1 L2 L3.
-Proof.
-  split; intro H; induction H; sauto.
-Qed.
+  (* Index-free update relation *)
+  Definition upd_rel_ex (l : lctx) (x y : R * A) (l' : lctx) : Prop :=
+    exists n, upd_rel l n x y l'.
 
-(* -------------------------------------------- *)
-(* Exhaustedness                                *)
-(* -------------------------------------------- *)
+  (* ---------------- Properties of lookup ---------------- *)
 
-Inductive exh {R A: Type} (hal : A -> Prop) : lctx R A -> Prop :=
-| exh_n : exh hal []
-| exh_c : forall {Δ : lctx R A} (X : R) {α : A},
-    exh hal Δ -> hal α -> exh hal ((X, α) :: Δ).
+  Lemma lookup_has_entry {l x} :
+    (exists n, lookup l n = Some x) <-> has_entry l x.
+  Proof. sauto use: nth_error_In, In_nth_error. Qed.
 
+  Lemma lookup_cons :
+    forall {Δ n A m} A' m',
+      lookup Δ n = Some (A, m) <->
+      lookup ((A', m') :: Δ) (S n) = Some (A, m).
+  Proof. intros; split; auto. Qed.
 
-Lemma exh_id  :
-  forall {A R} {join : Join A} {hal : A -> Prop} {Δ₁ Δ₂ Δ : lctx R A},
-    merge Δ₁ Δ₂ Δ ->
-    exh hal Δ₁ ->
+  Ltac impossible_lookup_nil :=
+    match goal with
+    | H : lookup [] _ = Some _ |- _ => assert (H' := nth_error_In _ _ H); inversion H'
+    end.
+  
+  (* ---------------- Properties of update ---------------- *)
+
+  Lemma upd_cons l n x y :
+    upd (x :: l) (S n) y = x :: (upd l n y).
+  Proof. constructor. Qed.
+
+  Lemma upd_head {l x y} :
+    upd (x :: l) 0 y = y :: l.
+  Proof. constructor. Qed.
+
+  Lemma upd_id {l n x} :
+    lookup l n = Some x -> upd l n x = l.
+  Proof. revert n; induction l; sauto. Qed.
+
+  Lemma upd_none {l n} :
+    lookup l n = None ->
+    forall x, upd l n x = l.
+  Proof. revert n; induction l; sauto. Qed.
+
+  Lemma upd_nil n x :
+    upd [] n x = [].
+  Proof. induction n; sauto. Qed.
+
+  Lemma upd_overwrite l n x y :
+    upd (upd l n x) n y = upd l n y.
+  Proof. revert n; induction l; sauto. Qed.
+
+  Lemma upd_comm {l n m x y} :
+    n <> m ->
+    upd (upd l n x) m y = upd (upd l m y) n x.
+  Proof.
+    revert l n m x y.
+    induction l as [|? ? IH]; intros n m ? ? ?.
+    - rewrite !upd_nil; reflexivity.
+    - destruct n, m; simpl; f_equal; [contradiction|apply IH; congruence].
+  Qed.
+
+  Lemma lookup_upd_eq :
+    forall {l n y} x,
+      lookup l n = Some y ->
+      lookup (upd l n x) n = Some x.
+  Proof.
+    induction l; intros n x y Hlk; destruct n; try discriminate.
+    - inversion Hlk; reflexivity.
+    - eapply IHl; exact Hlk.
+  Qed.
+
+  Lemma lookup_upd_neq {n m} :
+    n <> m ->
+    forall l y, lookup (upd l m y) n = lookup l n.
+  Proof. intros Hneq l. revert n m Hneq. induction l as [| ? ? ?]; intros; [|destruct n, m]; sauto. Qed.
+
+  (* ---------------- Properties of relational update ---------------- *)
+
+  (* `upd_rel` corresponds to lookup and update *)
+  Lemma upd_rel_iff_fun {l l' n x y} :
+    upd_rel l n x y l' <->
+    lookup l n = Some x /\ upd l n y = l'.
+  Proof. split; [intro H; induction H|revert n x y l'; induction l]; sauto. Qed.
+
+  Lemma lookup_upd_rel_neq {n m} :
+    n <> m ->
+    forall {l l' x y}, upd_rel l m x y l' -> lookup l' n = lookup l n.
+  Proof. intros; sauto using upd_rel_iff_fun, lookup_upd_neq. Qed.
+
+  Lemma upd_rel_refl {l l' n x} :
+    upd_rel l n x x l' -> l = l'.
+  Proof. intros H; dependent induction H. 2: f_equal; eapply IHupd_rel. all: eauto. Qed.
+
+  (* ---------------- Context merge ---------------- *)
+
+  Property merge_lookup {l1 l2 l3 n r a} :
+      lookup l3 n = Some (r, a) ->
+      join l1 l2 l3 ->
+      exists a1 a2,
+        join a1 a2 a /\
+        lookup l1 n = Some (r, a1) /\
+        lookup l2 n = Some (r, a2).
+  Proof.
+    intros Hlk Hm. revert n Hlk; induction Hm; intros ? Hlk.
+    - impossible_lookup_nil.
+    - destruct n.
+    + inversion Hlk; inversion H; exists (snd x), (snd y); repeat split; sauto.
+    + eapply IHHm in Hlk; destruct Hlk; eexists; repeat split; eauto.
+  Qed.
+
+  Corollary merge_has_entry {l1 l2 l3 r a} :
+      has_entry l3 (r, a) ->
+      join l1 l2 l3 ->
+      exists a1 a2,
+        join a1 a2 a /\
+        has_entry l1 (r, a1) /\
+        has_entry l2 (r, a2).
+  Proof.
+    intros Hin Hj.
+    destruct ((proj2 lookup_has_entry) Hin) as [? Hlk], (merge_lookup Hlk Hj) as (? & ? & ? & ? & ?).
+    repeat eexists; try (apply (proj1 lookup_has_entry); eexists); eassumption.
+  Qed.
+
+  Property merge_lookup_forward_l {l1 l2 l3 n r a1} :
+      lookup l1 n = Some (r, a1) ->
+      join l1 l2 l3 ->
+      exists a2 a,
+        join a1 a2 a /\
+        lookup l2 n = Some (r, a2) /\
+        lookup l3 n = Some (r, a).
+  Proof.
+    intros Hlk Hm; revert n Hlk; induction Hm; intros ? Hlk.
+    - impossible_lookup_nil.
+    - destruct n.
+    + inversion Hlk; subst; inversion H. exists (snd y), (snd z).
+      repeat split; simpl in *; sauto.
+    + eapply IHHm in Hlk; destruct Hlk; eexists; repeat split; eauto.
+  Qed.
+
+  Corollary merge_has_entry_forward_l {l1 l2 l3 r a1} :
+      has_entry l1 (r, a1) ->
+      join l1 l2 l3 ->
+      exists a2 a,
+        join a1 a2 a /\
+        has_entry l2 (r, a2) /\
+        has_entry l3 (r, a).
+  Proof.
+    intros Hin Hj.
+    destruct ((proj2 lookup_has_entry) Hin) as [? Hlk], (merge_lookup_forward_l Hlk Hj) as (? & ? & ? & ? & ?).
+    repeat eexists; try (apply (proj1 lookup_has_entry); eexists); eassumption.
+  Qed.
+
+  Property merge_lookup_forward_r {l1 l2 l3 n r a2} :
+      lookup l2 n = Some (r, a2) ->
+      join l1 l2 l3 ->
+      exists a1 a,
+        join a1 a2 a /\
+        lookup l1 n = Some (r, a1) /\
+        lookup l3 n = Some (r, a).
+  Proof. sauto use: merge_lookup_forward_l, join_comm. Qed.
+
+  Corollary merge_has_entry_forward_r {l1 l2 l3 r a2} :
+      has_entry l2 (r, a2) ->
+      join l1 l2 l3 ->
+      exists a1 a,
+        join a1 a2 a /\
+        has_entry l1 (r, a1) /\
+        has_entry l3 (r, a).
+  Proof. sauto use: merge_has_entry_forward_l, join_comm. Qed.
+
+  Lemma merge_lookup_none {l1 l2 l3 n} :
+    join l1 l2 l3 ->
+    (lookup l1 n = None <-> lookup l2 n = None) /\
+    (lookup l2 n = None <-> lookup l3 n = None).
+  Proof.
+    intros Hj; repeat split.
+    - intro H1.
+      destruct (lookup l2 n) as [[r a2]|] eqn:H2; auto.
+      destruct (merge_lookup_forward_r H2 Hj) as (a1 & a & _ & H1' & _).
+      rewrite H1 in H1'; discriminate.
+    - intro H2.
+      destruct (lookup l1 n) as [[r a1]|] eqn:H1; auto.
+      destruct (merge_lookup_forward_l H1 Hj) as (a2 & a & _ & H2' & _).
+      rewrite H2 in H2'; discriminate.
+    - intro H2.
+      destruct (lookup l3 n) as [[r a]|] eqn:H3; auto.
+      destruct (merge_lookup H3 Hj) as (a1 & a2 & _ & _ & H2').
+      rewrite H2 in H2'; discriminate.
+    - intro H3.
+      destruct (lookup l2 n) as [[r a2]|] eqn:H2; auto.
+      destruct (merge_lookup_forward_r H2 Hj) as (a1 & a & _ & _ & H3').
+      rewrite H3 in H3'; discriminate.
+  Qed.
+
+  (* If harmless elements are identity for resource join,
+    then exhausted contexts are identity for context join *)
+  Lemma exh_id {hal l1 l2 l} :
+    join l1 l2 l ->
+    exh hal l1 ->
     (forall a b c : A, join a b c -> hal a -> b = c) ->
-    Δ₂ = Δ.
-Proof.
-  intros. induction H; sauto.
-Qed.
+    l2 = l.
+  Proof. intros. induction H; sauto. Qed.
 
-(* -------------------------------------------- *)
-(* Update                                       *)
-(* -------------------------------------------- *)
+  Lemma merge_exh {hal l1 l2 l3} :
+    (forall a1 a2 a, join a1 a2 a -> hal a -> hal a1 /\ hal a2) ->
+    join l1 l2 l3 ->
+    exh hal l3 ->
+    exh hal l1 /\ exh hal l2.
+  Proof.
+    intros Hhal Hj Hexh; revert Hhal Hexh; induction Hj; intros Hhal Hexh.
+    - split; constructor.
+    - destruct H as [Hfst Hsnd], Hexh as [Hhal3 Hext],
+        (Hhal _ _ _ Hsnd Hhal3) as [Hh1 Hh2], (IHHj Hhal) as [IH1 IH2]; sauto.
+  Qed.
 
-Inductive updn {R A : Type} :
-  lctx R A -> nat -> R -> R -> A -> A -> lctx R A -> Prop :=
-| updn_t : forall (Δ : lctx R A) (X X' : R) (α α' : A),
-    updn ((X, α) :: Δ) 0 X X' α α' ((X', α') :: Δ)
-| updn_n : forall (Δ Δ' : lctx R A) (n : nat) (X X' Y : R) (α α' β : A),
-    updn Δ n X X' α α' Δ' ->
-    updn ((Y, β) :: Δ) (S n) X X' α α' ((Y, β) :: Δ').
+  Lemma merge_upd {l1 l2 l3 a a1 a2} n r :
+    join l1 l2 l3 ->
+    join a1 a2 a ->
+    join (upd l1 n (r, a1))
+         (upd l2 n (r, a2))
+         (upd l3 n (r, a)).
+  Proof.
+    intros * Hj Ha; revert n; induction Hj; intros n.
+    - sauto.
+    - destruct n; [sauto|constructor; [exact H|apply IHHj]].
+  Qed.
 
-(* w/o index *)
-Inductive upd {R A : Type}:
-  lctx R A -> R -> R -> A -> A -> lctx R A -> Prop :=
-| upd_t : forall (Δ : lctx R A) (X X' : R) (α α' : A),
-    upd ((X, α) :: Δ) X X' α α' ((X', α') :: Δ)
-| upd_n : forall (Δ Δ' : lctx R A) (X X' Y : R) (α α' β : A),
-    upd Δ X X' α α' Δ' ->
-    upd ((Y, β) :: Δ) X X' α α' ((Y, β) :: Δ').
+  (**
+    As a sanity check, we give an inductive characterization of lctx,
+    and show that it has the same action on the join relation. We should
+    not directly use this definition in any future developments, but
+    instead should use JoinFunctor_lctx applied to the resource algebra we are
+    annotating contexts with.
+  **)
 
-Property upd_exh_inv
-  {R A : Type} {hal : A -> Prop} {t s s' : R} {Δ Δ' α α'} :
-    upd ((t, α) :: Δ) s s' α α' Δ' ->
-    exh hal Δ' ->
-    ~ hal α -> hal α' ->
-    (s = t) /\ (Δ' = (s', α') :: Δ).
-Proof.
-  sauto.
-Qed.
+  Inductive merge_ind : Join lctx :=
+  | mg_n : merge_ind [] [] []
+  | mg_c r {l1 l2 l a1 a2 a} :
+      join a1 a2 a ->
+      merge_ind l1 l2 l ->
+      merge_ind ((r, a1) :: l1) ((r, a2) :: l2) ((r, a) :: l).
 
-(* -------------------------------------------- *)
-(* Permutations                                 *)
-(* -------------------------------------------- *)
+  Proposition merge_is_JoinFunctor_lctx {l1 l2 l3 : lctx}:
+    merge_ind l1 l2 l3 <-> join l1 l2 l3.
+  Proof. split; intro H; induction H; sauto. Qed.
 
-From Coq Require Import Sorting.Permutation.
+  (* ---------------- Permutations ---------------- *)
 
-Property perm_join {R A : Type} {JA : Join A} :
-  forall {Δ₁ Δ₂ Δ Δ' : lctx R A} ,
-    Permutation Δ Δ' ->
-    join Δ₁ Δ₂ Δ ->
-    exists Δ₁' Δ₂',
-      Permutation Δ₁ Δ₁' /\
-      Permutation Δ₂ Δ₂' /\
-      join Δ₁' Δ₂' Δ'.
-Proof.
-  intros Δ₁ Δ₂ Δ Δ' P M. revert Δ₁ Δ₂ M.
-  induction P; intros.
-  - (* perm_nil *)
-    inversion M. exists [], []. repeat split; constructor.
-  - (* perm_skip *)
-    inversion M as [ | x1 x2 ? ? ? ? ? M1].
-    destruct (IHP _ _ M1) as (Δ₁' & Δ₂' & ? & ? & ?).
-    exists (x1 :: Δ₁'), (x2 :: Δ₂').
-    repeat split; econstructor; auto.
-  - (* perm_swap *)
-    inversion M as [ | x1 x2 ? ? ? ? ?
-                   [ | y1 y2 ? Δ₁' Δ₂' ? ? ?]].
-    exists (y1 :: x1 :: Δ₁'), (y2 :: x2 :: Δ₂').
-    repeat split; constructor; sauto.
-  - (* perm_trans *)
-    destruct (IHP1 _ _ M) as (? & ? & ? & ? & M1).
-    destruct (IHP2 _ _ M1) as (Δ₁' & Δ₂' & ? & ? & ?).
-    exists Δ₁', Δ₂'.
-    repeat split; try eapply Permutation_trans; eauto.
-Qed.
+  Lemma lookup_perm {l l' n x} :
+    Permutation l l' ->
+    lookup l n = Some x ->
+    exists n', lookup l' n' = Some x.
+  Proof.
+    intros Hperm Hlk. revert n x Hlk.
+    induction Hperm; intros * Hlk.
+    - eauto.
+    - destruct n.
+      + inversion Hlk; exists 0; reflexivity.
+      + apply IHHperm in Hlk as [n' ?]; exists (S n'); assumption.
+    - destruct n as [|[|n']].
+      + inversion Hlk; exists 1; reflexivity.
+      + inversion Hlk; exists 0; reflexivity.
+      + exists (S (S n')); assumption.
+    - apply IHHperm1 in Hlk as [? H1]; apply IHHperm2 in H1 as [n' ?].
+      exists n'; assumption.
+  Qed.
 
-Lemma perm_upd :
-  forall {A R} {join : Join A} {Γ Γ' : lctx R A},
-    Permutation Γ Γ' ->
-    forall {A B α β Δ},
-      upd Γ A B α β Δ ->
-      exists Δ', Permutation Δ Δ' /\ upd Γ' A B α β Δ'.
-Proof.
-  intros. dependent induction H.
-  + (* nil *) strivial.
-  + (* skip *) sauto.
-  + (* swap *) sauto.
-  + (* trans *)
-    intros.
-    destruct (IHPermutation1 _ _ _ _ _ H1) as [? [? U]].
-    destruct (IHPermutation2 _ _ _ _ _ U) as [?Δ' [? ?]].
-    exists Δ'; hauto use: perm_trans.
-Qed.
+  Property perm_join l1 l2 l l' :
+    Permutation l l' ->
+    join l1 l2 l ->
+    exists l1' l2',
+      Permutation l1 l1' /\
+      Permutation l2 l2' /\
+      join l1' l2' l'.
+  Proof.
+    intros Hp Hj; revert l1 l2 Hj; induction Hp; intros.
+    - (* perm_nil *)
+      inversion Hj; subst; eauto.
+    - (* perm_skip *)
+      inversion Hj as [| x1 x2 ? ? ? ? ? Hj'].
+      destruct (IHHp _ _ Hj') as (l1' & l2' & ? & ? & ?).
+      repeat eexists; econstructor; eauto.
+    - (* perm_swap *)
+      inversion Hj as [| x1 x2 ? ? ? ? ? [| y1 y2 ? l1' l2' ? ? ?]].
+      exists (y1 :: x1 :: l1'), (y2 :: x2 :: l2').
+      repeat split; constructor; sauto.
+    - (* perm_trans *)
+      destruct (IHHp1 _ _ Hj) as (? & ? & ? & ? & Hj').
+      destruct (IHHp2 _ _ Hj') as (? & ? & ? & ? & ?).
+      repeat eexists; try eapply Permutation_trans; eauto.
+  Qed.
 
-Lemma perm_exh :
-  forall {A R} {join : Join A} {hal : A -> Prop} {Δ Δ' : lctx R A},
-    Permutation Δ Δ' ->
-    exh hal Δ ->
-    exh hal Δ'.
-Proof.
-  intros. induction H; sauto.
-Qed.
+  Lemma perm_upd {l l' n x} y :
+    Permutation l l' ->
+    lookup l n = x ->
+    exists m,
+      lookup l' m = x /\
+      Permutation (upd l n y) (upd l' m y).
+  Proof.
+    intros Hp; revert n x; induction Hp; intros n ? Hlk.
+    - (* perm_nil *)
+      destruct x.
+      + impossible_lookup_nil.
+      + exists n; eauto.
+    - (* perm_skip *)
+      destruct n; simpl in Hlk.
+      + inversion Hlk; exists 0; simpl; auto.
+      + specialize (IHHp _ _ Hlk) as (m & Hm & Hp'); exists (S m); simpl; auto.
+    - (* perm_swap *)
+      destruct n as [|[|n']]; simpl in Hlk; inversion Hlk.
+      + exists 1; split; constructor.
+      + exists 0; split; constructor.
+      + exists (S (S n')); split; auto; constructor.
+    - (* perm_trans *)
+      specialize (IHHp1 _ _ Hlk) as (m & Hm & Hp1').
+      specialize (IHHp2 _ _ Hm) as (k & Hk & Hp2').
+      exists k; split; auto. eapply perm_trans; eauto.
+  Qed.
+
+  Corollary perm_upd_rel {l1 l1' l2 n x y} :
+    Permutation l1 l2 ->
+    upd_rel l1 n x y l1' ->
+    exists m l2',
+      upd_rel l2 m x y l2' /\
+      Permutation l1' l2'.
+  Proof.
+    intros HP Hur. apply upd_rel_iff_fun in Hur as [Hlk Heq].
+    destruct (perm_upd y HP Hlk) as (m & ? & ?).
+    exists m, (upd l2 m y). sauto using upd_rel_iff_fun, Heq.
+  Qed.
+
+  Lemma perm_exh {hal l l'} :
+    Permutation l l' ->
+    exh hal l ->
+    exh hal l'.
+  Proof. intros. induction H; sauto. Qed.
+
+End ListCtx.
