case_studies/illc/typing_ext.v
@@ -22,116 +22,51 @@ Set Implicit Arguments.
 Inductive has_type {n} (Δ : tenv n) : tm n → ty → Prop :=
 
   | t_VarL :
-      forall (Δ' : tenv n) (T : ty) (fn : fin n),
+      ∀ (Δ' : tenv n) (T : ty) (fn : fin n),
         Δ fn = (T, one) →
-        exh _ _  _ hal (update_tfctx _ _ _ Δ fn T zero) →
+        exh hal (upd Δ fn (T, zero)) →
         has_type Δ (var_tm fn) T
 
   | t_VarI :
-      forall (T : ty) (fn : fin n),
+      ∀ (T : ty) (fn : fin n),
         Δ fn = (T, omega) →
-        @exh _ _ mult hal Δ →
+        exh hal Δ →
         has_type Δ (var_tm fn) T
 
   | t_Unit :
-        @exh _ _ mult hal Δ →
+        exh hal Δ →
         has_type Δ unit Unit
 
   | t_ElimUnit :
-      forall Δ1 Δ2 M N B,
+      ∀ Δ1 Δ2 M N B,
         has_type Δ1 M Unit →
         has_type Δ2 N B →
         join Δ1 Δ2 Δ →
         has_type Δ (elimunit M N) B
 
   | t_Abs :
-      forall (T1 T2 : ty) e1,
+      ∀ (T1 T2 : ty) e1,
         has_type (scons (T2, one) Δ) e1 T1 →
         has_type Δ (lam T2 e1) (Fun T2 T1)
 
   | t_App :
-      forall (Δ1 Δ2 : tenv n) (T1 T2 : ty) (e1 e2 : tm n),
+      ∀ (Δ1 Δ2 : tenv n) (T1 T2 : ty) (e1 e2 : tm n),
         has_type Δ1 e1 (Fun T2 T1) →
         has_type Δ2 e2 T2 →
         join Δ1 Δ2 Δ →
         has_type Δ (Core.app e1 e2) T1
 
   | t_Bang :
-      forall M A,
+      ∀ M A,
         has_type Δ M A →
         @exh _ _ mult hal Δ →
         has_type Δ (bang M) (Bang A)
 
   | t_LetBang :
-      forall Δ1 Δ2 M N A B,
+      ∀ Δ1 Δ2 M N A B,
         has_type Δ1 M (Bang A) →
         has_type (scons (A, omega) Δ2) N B →
         join Δ1 Δ2 Δ →
         has_type Δ (letbang M N) B.
 
 Notation "Δ '⊢' M ':' A" := (has_type Δ M A) (at level 40).
-
-(* ------------------------------------- *)
-(* Canonical forms lemma                 *)
-(* ------------------------------------- *)
-
-Lemma canonical_forms_fun :
-  forall (M : tm 0) T1 T2,
-    has_type emptyT M (Fun T1 T2) →
-    value M →
-    exists N U, M = (lam U N).
-Proof. sauto lq: on . Qed.
-  
-(* Canonical lemma for Unit *)
-Lemma canonical_forms_unit :
-  forall (M : tm 0),
-    has_type emptyT M Unit →
-    value M →
-    M = unit.
-Proof. sauto lq: on . Qed.
-
-(* Canonical form lemma for Bang *)
-Lemma canonical_forms_bang :
-  forall (M : tm 0) A,
-    has_type emptyT M (Bang A) →
-    value M →
-    exists N, M = bang N.
-Proof. sauto lq: on . Qed.
-
-(* ------------------------------------- *)
-(* Progress                              *)
-(* ------------------------------------- *)
-
-Lemma progress (M : tm 0) : forall T,
-  has_type emptyT M T → value M ∨ exists M', step M M'.  
-Proof.
-  dependent induction M; intros; try sfirstorder.
-  - (* elimunit *)
-    right. inversion H; subst.
-    apply join_emptyT in H5; sintuition.
-    destruct (IHM1 M1 eq_refl JMeq_refl Unit H2).
-     + (* t1 is a value *)
-      apply canonical_forms_unit in H2; [ | assumption]; subst.
-      destruct (IHM2 M2 eq_refl JMeq_refl T H3); [ | destruct H0]; eauto.
-    + (* t1 can step *)
-      destruct H0. eauto.
-  - (* app *)
-    right. inversion H; subst.
-    apply join_emptyT in H5; sintuition.
-    destruct (IHM1 M1 eq_refl JMeq_refl (Fun T2 T) H2).
-    + (* t1 is a value *)
-      apply canonical_forms_fun in H2; [ | assumption].
-      destruct H2 as [x [t H2]]; subst.
-      destruct (IHM2 M2 eq_refl JMeq_refl T2 H3); [ | destruct H0]; eauto.
-    + (* t1 can step *)
-      destruct H0. eauto.
-      - (* bang *) sauto.
-      - (* letbang *) right. inversion H; subst.
-    apply join_emptyT in H5; sintuition.
-    destruct (IHM1 M1 eq_refl JMeq_refl (Bang A) H2).
-    + (* t1 is a value *)
-      apply canonical_forms_bang in H2; [ | assumption].
-      sauto lq: on .
-    + (* t1 can step *)
-      destruct H0. eauto.
-Qed.
