case_studies/llc/typing.v
@@ -7,7 +7,7 @@
 From Coq Require Import Logic.FunctionalExtensionality Unicode.Utf8.
 From Hammer Require Import Tactics.
 From VST.msl Require Import sepalg.
-From CARVe Require Import contexts.total_fun algebras.purely_linear.
+From CARVe Require Import contexts.total_fun algebras.linear.
 From Autosubst Require Import fintype stlc step.
 Require Import tenv.
 Import ScopedNotations.
@@ -22,51 +22,21 @@ Set Implicit Arguments.
 Inductive has_type {n} (Δ : tenv n) : tm n → ty → Prop :=
 
 | t_Var :
-    forall (T : ty) (fn : fin n),
-      lookup_tfctx _ _ _ Δ fn = (T, one) ->
-      exh _ _  _ hal (update_tfctx _ _ _ Δ fn T zero) ->
+    ∀ (T : ty) (fn : fin n),
+      lookup Δ fn = (T, one) ->
+      exh hal (upd Δ fn (T, zero)) ->
       has_type Δ (var_tm fn) T
 
 | t_Abs :
-    forall (T1 T2 : ty) e1,
+    ∀ (T1 T2 : ty) e1,
       has_type (scons (T2, one) Δ) e1 T1 →
       has_type Δ (lam T2 e1) (Fun T2 T1)
 
 | t_App :
-    forall (Δ1 Δ2 : tenv n) (T1 T2 : ty) (e1 e2 : tm n),
+    ∀ (Δ1 Δ2 : tenv n) (T1 T2 : ty) (e1 e2 : tm n),
       has_type Δ1 e1 (Fun T2 T1) →
       has_type Δ2 e2 T2 →
       join Δ1 Δ2 Δ →
       has_type Δ (Core.app e1 e2) T1.
 
 Notation "Δ '⊢' e ':' T" := (has_type Δ e T) (at level 40).
-
-(* -------------------------------------------- *)
-(* Canonical forms lemma                        *)
-(* -------------------------------------------- *)
-
-Lemma canonical_forms_fun : forall (M : tm 0) T1 T2,
-  has_type emptyT M (Fun T1 T2) →
-  value M →
-  exists N U, M = (lam U N).
-Proof. sauto lq: on . Qed.
-
-(* -------------------------------------------- *)
-(* Progress                                     *)
-(* -------------------------------------------- *)
-
-Lemma progress (M : tm 0) : forall T,
-  has_type emptyT M T → value M ∨ exists M', step M M'.  
-Proof.
-  dependent induction M; intros; try sfirstorder.
-  - (* app case *)
-    right. inversion H; subst.
-    apply join_emptyT in H5; sintuition.
-    destruct (IHM1 M1 eq_refl JMeq_refl (Fun T2 T) H2).
-    + (* t1 is a value *)
-      apply canonical_forms_fun in H2; [ | assumption].
-      destruct H2 as [? [? ?]]; subst.
-      destruct (IHM2 M2 eq_refl JMeq_refl T2 H3); [ | destruct H0]; eauto.
-    + (* t1 can step *)
-      destruct H0. eauto.
-Qed.
