src/algebras/affine.v
@@ -1,0 +1,106 @@
+From Coq Require Import List Program.Equality Unicode.Utf8.
+From Hammer Require Import Tactics.
+From VST.msl Require Import sepalg.
+
+Inductive mult : Type :=
+| zero : mult  (* used *)
+| one  : mult. (* available at most once *)
+
+Inductive mult_op : mult -> mult -> mult -> Prop :=
+| m_00 : mult_op zero zero zero
+| m_10 : mult_op one zero one
+| m_01 : mult_op zero one one.
+
+Notation "c == a • b" := (mult_op a b c) (at level 50, left associativity).
+
+Instance Join_mult : Join mult := mult_op.
+
+Variant hal : mult → Prop :=
+| halz : hal zero
+| halo : hal one.
+
+Lemma mult_eq_dec : forall (X Y : mult), {X = Y} + {X <> Y}.
+Proof. decide equality. Qed.
+
+(* Monoidal properties *)
+(* Remark: `mult_hal_unit` does not hold, since not all harmless elements are unit *)
+
+Lemma mult_unit : forall a, exists u, mult_op u a a.
+Proof. intros. destruct a; hauto l: on . Qed.
+
+Lemma mult_op_comm : forall (a b c : mult), mult_op a b c -> mult_op b a c.
+Proof. sauto lq: on. Qed.
+
+Lemma mult_func : forall α₁ α₂ α α', mult_op α₁ α₂ α → mult_op α₁ α₂ α' → α = α'.
+Proof. sauto lq: on. Qed.
+
+Lemma mult_canc : forall α₁ α₂ α α₂', mult_op α₁ α₂ α → mult_op α₁ α₂' α → α₂ = α₂'.
+Proof. sauto lq: on. Qed.
+
+Instance mult_Canc_alg : @Canc_alg mult mult_op.
+Proof. unfold Canc_alg. sauto lq: on. Qed.
+
+Lemma mult_op_assoc : forall a b c d e,
+  mult_op a b d -> mult_op d c e ->
+  exists f, mult_op b c f /\ mult_op a f e.
+Proof. intros * H1 H2; inversion H1; subst; inversion H2; eauto using mult_op. Qed.
+
+Lemma join_positivity : forall a a' b b', mult_op a a' b -> mult_op b b' a -> a=b.
+Proof. sauto lq: on . Qed.
+
+Lemma mult_op_assoc' : forall a b c d e,
+  mult_op a b d -> mult_op d c e ->
+  {f : mult & mult_op b c f /\ mult_op a f e}.
+Proof.
+  intros a b c d e ? ?; destruct a, b, c, d, e;
+    try match goal with
+      | [ H : mult_op zero one zero |- _ ] => assert (~ mult_op zero one zero); [ unfold not; intro X; inversion X; auto | intuition]
+      | [ H : mult_op one zero zero |- _ ] => assert (~ mult_op one zero zero); [ unfold not; intro X; inversion X; auto | intuition]
+      | [ H : mult_op zero zero one |- _ ] => assert (~ mult_op zero zero one); [ unfold not; intro X; inversion X; auto | intuition]
+      | [ H : mult_op one one zero |- _ ] => assert (~ mult_op one one zero); [ unfold not; intro X; inversion X; auto | intuition]
+      | [ H : mult_op one one one |- _ ] => assert (~ mult_op one one one); [ unfold not; intro X; inversion X; auto | intuition]
+      | [ |- {f : mult & mult_op zero zero f /\ mult_op zero f zero } ] => eexists; exact (conj m_00 m_00)
+      | [ |- {f : mult & mult_op zero zero f /\ mult_op one f one } ] => eexists; exact (conj m_00 m_10)
+      | [ |- {f : mult & mult_op zero one f /\ mult_op zero f one } ] => eexists; exact (conj m_01 m_01)
+      | [ |- {f : mult & mult_op one zero f /\ mult_op zero f one } ] => eexists; exact (conj m_10 m_01)
+      end.
+Qed.
+
+Instance Perm_alg_mult : Perm_alg mult :=
+  @mkPerm mult Join_mult
+    mult_func        (* join_eq *)
+    mult_op_assoc'   (* join_assoc *)
+    mult_op_comm     (* join_comm *)
+    join_positivity. (* join_positivity *)
+
+(* Proving mult is a separation algebra *)
+
+Lemma mult_unit_sep : exists u, forall a, mult_op u a a.
+Proof. exists zero. intros. destruct a; hauto l: on . Qed.
+
+Lemma mult_unit_sep_unique : exists ! u, forall a, mult_op u a a.
+Proof. sauto lq: on use: mult_canc. Qed.
+
+Definition mult_op_sub (a c : mult) : Prop := exists b, mult_op a b c.
+Notation "a ⊑ c" := (mult_op_sub a c) (at level 70, no associativity).
+
+Definition mcore (m : mult) : mult :=
+  match m with
+  | zero => zero
+  | one => zero
+  end.
+
+Lemma mcore_unit: forall t, unit_for (mcore t) t.
+Proof. intros [|]; constructor. Qed.
+
+Lemma join_mcore_sub: forall (a b c : mult), mult_op a b c -> mult_op_sub (mcore a) (mcore c).
+Proof. sauto lq: on . Qed.
+
+Lemma mcore_idem : forall a, mcore (mcore a) = mcore a.
+Proof. intros [|]; reflexivity. Qed.
+
+Instance mult_Sep_alg : Sep_alg mult :=
+  { core := mcore;
+    core_unit := mcore_unit;
+    join_core_sub := join_mcore_sub;
+    core_idem := mcore_idem }.
