src/contexts/partial_fun.v
@@ -4,13 +4,11 @@ From CARVe Require Import optalg.
 
 (* Decidable equality *)
 Class EqDec (A : Type) : Type :=
-  {
-    eq_dec : forall x y : A, {x = y} + {x <> y}
-  }.
+  { eq_dec : forall x y : A, {x = y} + {x <> y} }.
 
 Section FunCtx.
   Variable R: Type.
-  Variable A: Type. (* Resource Algebra *)
+  Variable A: Type. (* Resource algebra *)
   Variable JA: Join A.
   Variable CA: Canc_alg A.
   Variable PA: Perm_alg A.
@@ -22,8 +20,7 @@ Section FunCtx.
     Join_fun _ _ (Join_opt _ JA).
 
   (* The following is only included to provide intuition on the fairly
-  opaque definition. It is not meant to be used in any
-  developments. *)
+  opaque definition. It is not meant to be used in any developments. *)
   Proposition _explicit_Join_fctx :
     forall C1 C2 C3,
       join C1 C2 C3 <-> (forall x,
@@ -32,22 +29,14 @@ Section FunCtx.
                           | None, None, None => True
                           | _, _, _ => False
                           end).
-  Proof.
-    reflexivity.
-  Qed.
+  Proof. reflexivity. Qed.
 
   #[global] Instance Perm_alg_fctx : Perm_alg fctx.
-  Proof.
-    hauto use: Perm_fun, Perm_opt.
-  Defined.
+  Proof. hauto use: Perm_fun, Perm_opt. Defined.
   #[global] Instance Canc_alg_fctx : Canc_alg fctx.
-  Proof.
-    hauto use: Canc_fun, Canc_opt.
-  Defined.
+  Proof. hauto use: Canc_fun, Canc_opt. Defined.
   #[global] Instance Sep_alg_fctx : Sep_alg fctx.
-  Proof.
-    hauto use: Sep_fun, Sep_opt, Perm_opt.
-  Defined.
+  Proof. hauto use: Sep_fun, Sep_opt, Perm_opt. Defined.
 
   Definition exh (hal: A -> Prop): fctx -> Prop :=
     fun C => forall r, match C r with
@@ -65,4 +54,5 @@ Section FunCtx.
 
   Definition is_defined : fctx -> R -> Prop :=
     fun C r => C r <> None.
+
 End FunCtx.
