case_studies/closures/README.md
@@ -1,8 +1,8 @@
 # Closures
 
 This subdirectory contains various versions of weak normalization for a closure-based
-presentation of the linear lambda calculus.
-The encoding is based on standard de Bruijn notation (not well scoped).
+presentation of the linear λ-calculus.
+The encoding is based on standard de Bruijn notation (not well-scoped).
 The operational semantics is big-step and does not perform substitutions, so no shifting nor substitution lemmas are required.
 
 ## Files
@@ -13,4 +13,4 @@ The operational semantics is big-step and does not perform substitutions, so no 
 
 - **basicIclo.v**:  
   Intrinsically-typed DB version, but **not** linear. 
-  Meant as a stepping stone toward a fully linear version.
+  Meant as a stepping stone toward a future fully linear version.
